More work on lattices

coq/Lattice.v
@@ -1,23 +1,25 @@
 Require Import Coq.Program.Program.
 Require Import Coq.Bool.Bool.
 Require Import Coq.Arith.Bool_nat.
+Require Import Coq.Arith.PeanoNat.
 Require Import Coq.Lists.List.
 Require Import Coq.Relations.Relations.
 Require Import Coq.Classes.RelationClasses.
+Require Import Coq.quote.Quote.
 
 Generalizable All Variables.
 
 Reserved Infix "⊓" (at level 40, left associativity).
 Reserved Infix "⊔" (at level 36, left associativity).
 
-Class Lattice (A : Type) := {
+Class Lattice (A : Set) := {
   meet : A -> A -> A where "x ⊓ y" := (meet x y);
   join : A -> A -> A where "x ⊔ y" := (join x y);
 
   meet_commutative : forall a b, a ⊓ b = b ⊓ a;
   meet_associative : forall a b c, (a ⊓ b) ⊓ c = a ⊓ (b ⊓ c);
   meet_absorptive  : forall a b, a ⊓ (a ⊔ b) = a;
-  meet_idempotent  : forall a,  a ⊓ a = a;
+  meet_idempotent  : forall a, a ⊓ a = a;
 
   join_commutative : forall a b, a ⊔ b = b ⊔ a;
   join_associative : forall a b c, (a ⊔ b) ⊔ c = a ⊔ (b ⊔ c);
@@ -28,7 +30,7 @@ Class Lattice (A : Type) := {
 Infix "⊓" := meet (at level 40, left associativity).
 Infix "⊔" := join (at level 36, left associativity).
 
-Class Order (A : Type) := {
+Class Order (A : Set) := {
   ord : relation A;
 
   reflexive :> Reflexive ord;
@@ -44,6 +46,8 @@ Class LOSet (A : Set) := {
   consistent: forall a b, a ≤ b <-> a = a ⊓ b
 }.
 
+Coercion is_lattice {A : Set} (O : LOSet A) : Lattice A := lattice.
+
 Section Lattice.
 
 Context `{l : LOSet A}.
@@ -58,17 +62,75 @@ Proof.
     apply consistent.
     rewrite <- meet_associative, <- H0.
     assumption.
-Admitted.
+  apply consistent in H.
+  rewrite H; clear H.
+  split; apply consistent.
+    rewrite meet_associative.
+    f_equal.
+    rewrite meet_associative.
+    rewrite (meet_commutative b a).
+    rewrite <- meet_associative.
+    rewrite meet_idempotent.
+    reflexivity.
+  rewrite meet_associative.
+  f_equal.
+  rewrite meet_associative.
+  rewrite meet_idempotent.
+  reflexivity.
+Qed.
 
 Theorem join_is_lub : forall a b : A,
   forall x, a ≤ x /\ b ≤ x <-> a ⊔ b ≤ x.
 Proof.
+  split; intros.
+    intuition.
+    apply consistent in H0.
+    apply consistent in H1.
+    apply consistent.
 Admitted.
 
-Inductive Term (A : Type) : Set :=
+Set Decidable Equality Schemes.
+
+Inductive Term : Set :=
   | Var  : nat  -> Term
   | Meet : Term -> Term -> Term
   | Join : Term -> Term -> Term.
+
+Lemma Meet_acc_l x y : Meet x y <> x.
+Proof.
+  induction x;
+  unfold not; intros;
+  try discriminate.
+  inversion H; subst.
+  contradiction.
+Qed.
+
+Lemma Meet_acc_r x y : Meet x y <> y.
+Proof.
+  induction y;
+  unfold not; intros;
+  try discriminate.
+  inversion H; subst.
+  contradiction.
+Qed.
+
+Lemma Join_acc_l x y : Join x y <> x.
+Proof.
+  induction x;
+  unfold not; intros;
+  try discriminate.
+  inversion H; subst.
+  contradiction.
+Qed.
+
+Lemma Join_acc_r x y : Join x y <> y.
+Proof.
+  induction y;
+  unfold not; intros;
+  try discriminate.
+  inversion H; subst.
+  contradiction.
+Qed.
 
 Fixpoint length (t : Term) : nat :=
   match t with
@@ -86,9 +148,99 @@ Fixpoint depth (t : Term) : nat :=
 
 Inductive Subterm : Term -> Term -> Prop :=
   | Meet1 : forall t1 t2, Subterm t1 (Meet t1 t2)
-  | Meet2 : forall t1 t2, Subterm t2 (Meet t1 t2)
+  | Meet2 : forall t1 t2, t1 <> t2 -> Subterm t2 (Meet t1 t2)
   | Join1 : forall t1 t2, Subterm t1 (Join t1 t2)
-  | Join2 : forall t1 t2, Subterm t2 (Join t1 t2).
+  | Join2 : forall t1 t2, t1 <> t2 -> Subterm t2 (Join t1 t2).
+
+Definition Subterm_inv_t : forall x y, Subterm x y -> Prop.
+Proof.
+  intros [] [] f;
+  match goal with
+  | [ H : Subterm ?X (Meet ?X ?Z) |- Prop ] =>
+    exact (f = Meet1 _ _)
+  | [ H : Subterm ?X (Join ?X ?Z) |- Prop ] =>
+    exact (f = Join1 _ _)
+  | [ H : Subterm ?X (Meet ?Y ?Z) |- Prop ] =>
+    destruct (Term_eq_dec Y X) as [e|e]; subst;
+    [ exact (f = Meet1 _ _)
+    | destruct (Term_eq_dec X Z); subst;
+      [ exact (f = Meet2 Y X e)
+      | exact False ] ]
+  | [ H : Subterm ?X (Join ?Y ?Z) |- Prop ] =>
+    destruct (Term_eq_dec Y X) as [e|e]; subst;
+    [ exact (f = Join1 _ _)
+    | destruct (Term_eq_dec X Z); subst;
+      [ exact (f = Join2 Y X e)
+      | exact False ] ]
+  | _ => exact False
+  end.
+Defined.
+
+Theorem UIP_dec_not : forall (A : Type),
+  (forall x y:A, {x = y} + {x <> y}) ->
+  forall (x y:A) (p1 p2:x <> y), p1 = p2.
+Proof.
+  intros.
+  unfold not in *.
+  (* jww (2017-06-10): Is there any way to avoid an axiom here? *)
+  Require Import FunctionalExtensionality.
+  extensionality p.
+  subst; contradiction.
+Qed.
+
+Print Assumptions UIP_dec_not.
+
+Corollary Subterm_inv x y f : Subterm_inv_t x y f.
+Proof.
+  pose proof Term_eq_dec.
+  destruct f, t1, t2; simpl;
+  repeat destruct (Term_eq_dec _ _); subst;
+  unfold eq_rect_r;
+  try (rewrite e || rewrite <- e);
+  try congruence;
+  try rewrite <- Eqdep_dec.eq_rect_eq_dec; eauto;
+  f_equal;
+  apply UIP_dec_not; auto.
+Qed.
+
+Program Instance Subterm_StrictOrder : StrictOrder Subterm.
+Next Obligation.
+  repeat intro.
+  pose proof (Subterm_inv _ _ H).
+  inversion H; subst; simpl in *.
+  - now apply (Meet_acc_l x t2).
+  - now apply (Meet_acc_r t1 x).
+  - now apply (Join_acc_l x t2).
+  - now apply (Join_acc_r t1 x).
+Qed.
+Next Obligation.
+  repeat intro.
+  pose proof (Subterm_inv _ _ H).
+  pose proof (Subterm_inv _ _ H0).
+  inversion H; subst; simpl in *;
+  inversion H0; subst; simpl in *.
+  (* jww (2017-06-10): At least the way that Subterm is currently defined, it
+     is not transitive. *)
+Admitted.
+
+Lemma Subterm_wf : well_founded Subterm.
+Proof.
+  constructor; intros.
+  inversion H; subst; simpl in *.
+  - induction y, t2; simpl in *;
+    constructor; intros;
+    inversion H0; subst; clear H0;
+    try (apply IHy1; constructor);
+    try (apply IHy2; constructor).
+  - induction y, t1; simpl in *;
+    constructor; intros;
+    inversion H1; subst; clear H1.
+    destruct y1.
+    destruct (Term_eq_dec (Var n) (Var n0)).
+    apply IHy1.
+    constructor.
+    try (apply IHy1; constructor);
+    try (apply IHy2; constructor).
 
 Reserved Notation "〚 t 〛 env" (at level 9).
 
@@ -99,24 +251,18 @@ Fixpoint eval (t : Term) (env : nat -> A) : A :=
   | Join t1 t2 =>〚t1〛env ⊔〚t2〛env
   end where "〚 t 〛 env" := (eval t env).
 
-Fixpoint interp (t : Term) : A :=
-  match t with
-  | Var v => v
-  | Meet t1 t2 => interp t1 ⊓ interp t2
-  | Join t1 t2 => interp t1 ⊔ interp t2
-  end.
-
 Definition Leq   (s t : Term) : Prop := forall env, 〚s〛env ≤ 〚t〛env.
 Definition Equiv (s t : Term) : Prop := forall env, 〚s〛env = 〚t〛env.
 
 Reserved Infix "≲" (at level 30).
 
 Definition R := symprod Term Term Subterm Subterm.
+Arguments R /.
 
 Open Scope lazy_bool_scope.
 
 Program Fixpoint leq (p : Term * Term) {wf R p} :
-  { b : bool | Is_true b -> Leq (fst p) (snd p) } :=
+  { b : bool | b = true -> Leq (fst p) (snd p) } :=
   match p with
   | (s, t) =>
     let leqb x y := proj1_sig (leq (x, y)) in
@@ -130,6 +276,22 @@ Program Fixpoint leq (p : Term * Term) {wf R p} :
     end
   end where "s ≲ t" := (leq (s, t)).
 Next Obligation.
+  destruct (leq (x, t1)).
+    constructor.
+    admit.
+  simpl in *.
+  unfold Leq in l0.
+   apply left_sym.
+Admitted.
+Next Obligation.
+  unfold Leq; intros; simpl.
+  destruct (nat_eq_bool i j) eqn:Heqe; simpl in H; subst.
+  rewrite y.
+  reflexivity.
+Qed.
+Next Obligation.
+  unfold Leq; intros; simpl.
+  inversion Heq_p; subst.
 Admitted.
 Next Obligation.
 Admitted.
@@ -150,54 +312,102 @@ Admitted.
 Next Obligation.
 Admitted.
 Next Obligation.
+  unfold MR, R; simpl.
 Admitted.
-Next Obligation.
-Admitted.
-Next Obligation.
-Admitted.
+
+Notation "s ≲ t" := (leq (s, t)).
 
 Import ListNotations.
 
-Ltac intern vars e :=
-  let rec loop n vars' :=
-    match vars' with
-    | [] =>
-      let vars'' := eval simpl in (vars ++ [e]) in
-      constr:((n, vars''))
-    | e :: ?vars'' => constr:((n, vars))
-    | _ :: ?vars'' => loop (S n) vars''
-    end in
-  loop 0 vars.
+Ltac inList x xs :=
+  match xs with
+  | tt => false
+  | (x, _) => true
+  | (_, ?xs') => inList x xs'
+  end.
 
-Ltac reflect env m j t :=
+Ltac addToList x xs :=
+  let b := inList x xs in
+  match b with
+  | true => xs
+  | false => constr:((x, xs))
+  end.
+
+Ltac allVars xs m j e :=
+  match e with
+  | m ?e1 ?e2 =>
+    let xs := allVars xs m j e1 in
+    allVars xs m j e2
+  | j ?e1 ?e2 =>
+    let xs := allVars xs m j e1 in
+    allVars xs m j e2
+  | _ => addToList e xs
+  end.
+
+Ltac lookup x xs :=
+  match xs with
+  | (x, _) => O
+  | (_, ?xs') =>
+    let n := lookup x xs' in
+    constr:(S n)
+  end.
+
+Ltac reifyTerm env m j t :=
   match t with
-  | (m ?X1 ?X2) =>
-    let r1 := reflect env m j X1
-      with r2 := reflect env m j X2 in
+  | m ?X1 ?X2 =>
+    let r1 := reifyTerm env m j X1 in
+    let r2 := reifyTerm env m j X2 in
     constr:(Meet r1 r2)
-  | (j ?X1 ?X2) =>
-    let r1 := reflect env m j X1
-      with r2 := reflect env m j X2 in
+  | j ?X1 ?X2 =>
+    let r1 := reifyTerm env m j X1 in
+    let r2 := reifyTerm env m j X2 in
     constr:(Join r1 r2)
-  (* | ?X1 => *)
-  (*   let n := inv_lookup env X1 in *)
-  (*   constr:(Var n) *)
+  | ?X =>
+    let n := lookup X env in
+    constr:(Var n)
   end.
 
 Lemma leq_correct : forall t u : Term,
-  Is_true (` (leq (t, u))) -> forall env,〚t〛env ≤〚u〛env.
+  Is_true (` (t ≲ u)) -> forall env, 〚t〛env ≤ 〚u〛env.
 Proof.
+  intros.
+  induction t, u; simpl in *.
 Admitted.
+
+Ltac functionalize xs :=
+  let rec loop n xs' :=
+    match xs' with
+    | (?x, tt) => constr:(fun _ : nat => x)
+    | (?x, ?xs'') =>
+      let f := loop (S n) xs'' in
+      constr:(fun m : nat => if m =? n then x else f m)
+    end in
+  loop 0 xs.
+
+Ltac reify m j :=
+  match goal with
+  | [ |- ?S ≤ ?T ] =>
+    let xs  := allVars tt m j S in
+    let xs' := allVars xs m j T in
+    let r1  := reifyTerm xs' m j S in
+    let r2  := reifyTerm xs' m j T in
+    let env := functionalize xs' in
+    pose xs';
+    pose env;
+    pose r1;
+    pose r2;
+    change (〚r1〛env ≤ 〚r2〛env);
+    apply leq_correct;
+    vm_compute
+  end.
+
+Ltac lattice := reify meet join.
 
 Lemma median_inequality : forall x y z : A,
   (x ⊓ y) ⊔ (y ⊓ z) ⊔ (z ⊓ x) ≤ (x ⊔ y) ⊓ (y ⊔ z) ⊓ (z ⊔ x).
 Proof.
   intros.
-  destruct l.
-  reflect (fun n : nat => A) meet join ((x ⊓ y) ⊔ (y ⊓ z) ⊔ (z ⊓ x) ≤ x ⊔ y ⊓ y ⊔ z ⊓ z ⊔ x).
-  evar (env : nat -> A).
-  change ((x ⊓ y) ⊔ (y ⊓ z) ⊔ (z ⊓ x) ≤ x ⊔ y ⊓ y ⊔ z ⊓ z ⊔ x)
-    with (〚(x ⊓ y) ⊔ (y ⊓ z) ⊔ (z ⊓ x)〛env ≤〚x ⊔ y ⊓ y ⊔ z ⊓ z ⊔ x〛env).
+  lattice.
 Admitted.
 
 End Lattice.
